reorg files; add test case; fix transpose operator

Tensor/Basic.lean
@@ -1,182 +1,9 @@
+-- Scott Kovach
 import Init.Data.Array.Subarray
 import Init.Data.Float
-import Tensor.Order
-import Tensor.Enumerable
+import Std.Data.RBMap
+import Tensor.Has
 
-section Util
-def range (n : Nat) : List Nat := do
-    let mut result := []
-    for x in [0:n] do
-        result := x :: result
-    return result.reverse
-end Util
-
-class HasZero (α : Type _) where zero : α
-class HasOne (α : Type _) where one : α
-instance : HasZero Nat where zero := 0
-instance : HasOne  Nat where one := 1
-instance : HasZero Float where zero := 0.0
-instance : HasOne  Float where one := 1.0
-
-/-- A function-backed vector -/
-structure Vec (ι : Type u) (α : Type v) where
-    toFun : ι → α
-
-macro "vec" xs:Lean.explicitBinders " => " b:term : term => Lean.expandExplicitBinders `Vec.mk xs b
-
-/-- support `v[i]` notation. -/
-@[inline] def Vec.getOp (self : Vec ι α) (idx : ι) : α := self.toFun idx
-
-/-- A vector as a function mapping indices to values. -/
-class HasVec (β : Type u) (ι : outParam $ Type v) (α : outParam $ Type w) where
-    toVec : β → Vec ι α
-export HasVec (toVec)
-
-instance : HasVec (Vec ι α) ι α := ⟨ id ⟩
-
-instance [Add α] : Add (Vec ι α) where
-    add v w := vec i => v[i] + w[i]
-instance [Sub α] : Sub (Vec ι α) where
-    sub v w := vec i => v[i] - w[i]
-instance [Mul α] : Mul (Vec ι α) where
-    mul v w := vec i => v[i] * w[i]
-instance [Div α] : Div (Vec ι α) where
-    div v w := vec i => v[i] / w[i]
-
-namespace Vec
-
-def push (v : Vec ι (Vec κ α)) : Vec (ι × κ) α := vec p => v[p.1][p.2]
-def pop (v : Vec (ι × κ) α) : Vec ι (Vec κ α) := vec i j => v[(i, j)]
-def reindex (v : Vec ι α) (f : κ → ι) : Vec κ α := vec i => v[f i]
-
-instance : Monad (Vec ι) where
-    pure x := vec i => x
-    map f v := vec i => f v[i]
-    seq f v := vec i => f[i] v[i]
-    bind v f := vec i => (f v[i])[i] -- diagonal (is this actually a monad law?)
-
-instance [OfNat α n] : OfNat (Vec ι α) n where
-    ofNat := vec i => OfNat.ofNat n
-
-def transpose (v : Vec ι (Vec κ α)) : Vec κ (Vec ι α) := vec j i => v[i][j]
-
-end Vec
-
-def Vec.sum [Enumerable ι] [Add α] [OfNat α Nat.zero] (v : Vec ι α) : α := do
-    let mut s : α := 0
-    for i in Enumerable.listOf ι do
-        s := s + v[i]
-    return s
-
-structure DenseVec (ι : Type u) [Enumerable ι] (α : Type v) where
-    array : Array α
-    hasSize : array.size = Enumerable.card ι
-
-namespace DenseVec
-variable {ι : Type u} [Enumerable ι] {α : Type v}
-
-instance [Repr α] : Repr (DenseVec ι α) where
-    reprPrec d _ := repr d.array
-
-theorem sizeMapEq (a : Array α) (f : α → β) : (a.map f).size = a.size := sorry
-
-instance [HMul α α₁ α₁] : HMul α (DenseVec ι α₁) (DenseVec ι α₁) where
-    hMul r u := ⟨ u.array.map (λ x => r * x) , (sizeMapEq _ _).symm ▸ u.hasSize⟩
-
-#check Array
-#check Array.size_mkArray
-def fill (a : α) : DenseVec ι α where
-    array := Array.mkArray (Enumerable.card ι) a
-    hasSize := Array.size_mkArray ..
-
-def empty [Inhabited α] : DenseVec ι α :=
-    fill Inhabited.default
-
-def translateIdx (v : DenseVec ι α) (i : ι) : Fin v.array.size :=
-    let ⟨n, h⟩ := Enumerable.enum i
-    ⟨n, by rw v.hasSize; exact h⟩
-
-/-- Get the value associated to a particular index. -/
-def get (v : DenseVec ι α) (i : ι) : α :=
-    v.array.get (v.translateIdx i)
-
-/-- support `v[i]` notation. -/
-@[inline] def getOp (self : DenseVec ι α) (idx : ι) : α := self.get idx
-
-instance : HasVec (DenseVec ι α) ι α where
-    toVec v := vec i => v[i]
-
-def of [HasVec β ι α] (v : β) : DenseVec ι α where
-    array := do
-        let v' := toVec v
-        let mut a := Array.empty
-        for i in Enumerable.listOf ι do
-            a := a.push $ v'[i]
-        return a
-    hasSize := sorry -- need to define differently to be able to easily prove this
-
-/-- Set the value associated to a particular index. -/
-def set (v : DenseVec ι α) (i : ι) (a : α) : DenseVec ι α where
-    array := v.array.set (v.translateIdx i) a
-    hasSize := by rw [Array.size_set, v.hasSize]
-
-def forIn {α : Type u} {β : Type v} {m : Type v → Type w} [Monad m] (as : DenseVec ι α) (b : β) (f : α → β → m (ForInStep β)) : m β :=
-    as.array.forIn b f
-
-
-instance [HasZero α] [Enumerable ι] : HasZero (DenseVec ι α) where
-    zero := ⟨ Array.mkArray (Enumerable.card ι) HasZero.zero, Array.size_mkArray .. ⟩
-instance [HasZero α] [Enumerable ι] : OfNat (DenseVec ι α) 0 where
-    ofNat := HasZero.zero
-
-def pure (x : α) : DenseVec ι α := fill x
-
--- Kyle's add/dot
--- def dot (v w : DenseVec ι Float) : Float := do
---     let mut s : Float := 0
---     for i in Enumerable.listOf ι do
---         s := s + v[i] * w[i]
---     return s
--- def add [Add α] (v w : DenseVec ι α) : DenseVec ι α := do
---     let mut v := v
---     for i in Enumerable.listOf ι do
---         v := v.set i (v.get i + w.get i)
---     return v
-
-def add [Add α] [Inhabited α] ( u v : DenseVec ι α) : DenseVec ι α := do
-    let mut u := u.array
-    for i in [0:u.size] do
-        u := u.set! i (u[i] + v.array[i])
-    return ⟨ u , sorry⟩
-
-instance [Add α] [Inhabited α]: Add (DenseVec ι α) where
-    add := add
-
-end DenseVec
-
-theorem List.toArraySizeEq (x : List α) : x.toArray.size = x.length := sorry
--- theorem List.toArraySizeEq (x : List α) : x.toArray.size = x.length := by
---     hm; induction x; exact rfl; rw List.lengthConsEq;
-    -- rw Array.sizePushEq
-
-def List.toDenseVec (x : List α) : DenseVec (Fin x.length) α where
-    array := x.toArray
-    hasSize := List.toArraySizeEq ..
-
-syntax "![" sepBy(term, ", ") "]" : term
-
-macro_rules
-  | `(![ $elems,* ]) => `(List.toDenseVec [ $elems,* ])
-
-example : DenseVec (Fin 3) Nat := ![2,22,222]
-
-open Enumerable
-
-
-open PreOrder
-
-
--- TODO might as well have two type parameters
 inductive EitherOr (α β : Type _)
 | left : α → EitherOr α β
 | right : β → EitherOr α β
@@ -194,38 +21,10 @@ def reduce (unit : α) (op : α → α → α) : EitherOr α α → α
 | EitherOr.right y => op unit  y
 | EitherOr.both x y => op x y
 end EitherOr
+
 open EitherOr
 
---[s: LinearOrder β] [DecidableRel s.LessEq]
--- def merge_aux [DecidableEq β] [HasLessEq β] [DecidableRel (. ≤ . : β → β → Prop)] : Nat → List (β × α) → List (β × α) → List (β × EitherOr α)
--- | 0, _, _ => []
--- | (n+1), [], ys => ys.map λ ⟨i, a⟩ => ⟨i, right a⟩
--- | (n+1), xs, [] => xs.map λ ⟨i, a⟩ => ⟨i, left a⟩
--- | (n+1), l1@(⟨i, x⟩ :: xs), l2@(⟨j, y⟩ :: ys) =>
---     if i = j then
---         ⟨i, both x y⟩ :: merge_aux n xs ys
---     else if i ≤ j then
---         ⟨i, left x⟩ :: merge_aux n xs l2
---     else
---         ⟨j, right y⟩ :: merge_aux n l1 ys
-
--- reversed order!
-def merge_aux_aux [DecidableEq β] [HasLessEq β] [DecidableRel (. ≤ . : β → β → Prop)] : Nat → List (β × α) → List (β × α) →
-    List (β × EitherOr α α) → List (β × EitherOr α α)
-| 0, _, _, acc => acc
-| (n+1), [], ys, acc => ys.foldl (λ acc (i, a) => (i, right a) :: acc) acc
-| (n+1), xs, [], acc => xs.foldl (λ acc (i, a) => (i, left a) :: acc) acc
-| (n+1), l1@(⟨i, x⟩ :: xs), l2@(⟨j, y⟩ :: ys), acc =>
-    if i = j then
-        merge_aux_aux n xs ys (⟨i, both x y⟩ :: acc)
-    else if i ≤ j then
-        merge_aux_aux n xs l2 (⟨i, left x⟩ :: acc)
-    else
-        merge_aux_aux n l1 ys ((j, right y) :: acc)
-
--- def mergeOrList [DecidableEq β] [HasLessEq β] [DecidableRel (. ≤ . : β → β → Prop)] : Nat → List (β × α) → List (β × α) → List (β × EitherOr α α)
--- |  n, xs, ys => merge_aux_aux n xs ys [] |> List.reverse
-
+-- could have used `partial def`
 def mergeUnion [DecidableEq β] [le : HasLessEq β] [DecidableRel le.LessEq] :
     Nat → List (β × α) → List (β × α₁) → Array (β × EitherOr α α₁) → Array (β × EitherOr α α₁)
 | 0, _, _, acc => acc
@@ -239,18 +38,6 @@ def mergeUnion [DecidableEq β] [le : HasLessEq β] [DecidableRel le.LessEq] :
     else
         mergeUnion n l1 ys (acc.push (j, right y))
 
--- def merge'' [DecidableEq β] [HasLessEq β] [DecidableRel (. ≤ . : β → β → Prop)] (xs : List (β × α)) (ys : List (β × α)) : List (β × EitherOr α) :=
--- merge_aux_aux (xs.length + ys.length) xs ys []
-
---#eval Functor.map (\la
--- def mergeSum [Add α] [DecidableEq β] [HasLessEq β] [DecidableRel (. ≤ . : β → β → Prop)] (xs : List (β × α)) (ys : List (β × α)) : List (β × α) :=
--- (merge' xs ys).map λ (b, m) => (b, reduce m)
--- def mergeSum' [Add α] [DecidableEq β] [HasLessEq β] [DecidableRel (. ≤ . : β → β → Prop)] (xs : Array (β × α)) (ys : Array (β × α)) : Array (β × α) := do
---     let mut res := Array.empty
---     for p in merge_aux (xs.size + ys.size) xs.toList ys.toList do
---         res := res.push ⟨p.1, reduce p.2⟩
---     return res
-
 def scaleArray [HMul α α₁ α₁] (r: α) (u : Array α₁) : Array α₁ :=
     u.map (λ x => r * x)
 
@@ -261,10 +48,10 @@ def SparseVec ι α := Array (ι × α)
 
 namespace SparseVec
 
-instance [r : Repr (Array (ι × α))] : Repr (SparseVec ι α) := ⟨ r.reprPrec ⟩
-instance [r : ToString (Array (ι × α))] : ToString (SparseVec ι α) := ⟨ r.toString ⟩
+-- needed without `reducible` attribute (also needs ForIn)
+-- instance [r : Repr (Array (ι × α))] : Repr (SparseVec ι α) := ⟨ r.reprPrec ⟩
+-- instance [r : ToString (Array (ι × α))] : ToString (SparseVec ι α) := ⟨ r.toString ⟩
 
-def exAdd1 := ()
 def sparseAdd [s : Add α] [u : HasZero α] [DecidableEq β] [le : HasLessEq β] [DecidableRel le.LessEq]
     (xs ys : SparseVec β α ) : SparseVec β α := do
     let mut res := Array.empty
@@ -272,7 +59,7 @@ def sparseAdd [s : Add α] [u : HasZero α] [DecidableEq β] [le : HasLessEq β]
         res := res.push (coord, EitherOr.reduce u.zero s.add values)
     return res
 
-#reduce λ a b => sparseAdd #[(1, a), (2, 3)] #[(1,b),(2,1)]
+#eval sparseAdd #[(1, 3), (5, 4)] #[(1,5),(2,1)]
 
 def map (f : α → β) (v : SparseVec ι α) : SparseVec ι β :=
     Array.map (λ (c, x) => (c, f x)) v
@@ -324,15 +111,14 @@ instance [DecidableEq ι] [le : HasLessEq ι] [DecidableRel le.LessEq]
     : HMul (SparseVec Nat (SparseVec ι α)) (SparseVec ι β) (SparseVec Nat β) :=
     ⟨ linearCombinationOfRows ⟩
 
-def sparseTranspose (n : Nat) (A : SparseVec Nat (SparseVec Nat α)) : SparseVec Nat (SparseVec Nat α) := do
-    let mut out := Array.mkArray n (0, #[])
-    for (rowC, row) in A do
-        for (coord, value) in row do
-            out := Array.set! out (coord-1) (coord, out[coord-1].2.push (rowC, value))
-    return out
+def sparseTranspose (A : SparseVec Nat (SparseVec Nat α)) : SparseVec Nat (SparseVec Nat α) := do
+  let mut temp := Std.mkRBMap Nat (SparseVec Nat α) (. < .)
+  for (rowC, row) in A do
+    for (coord, value) in row do
+      temp := temp.insert coord (temp.findD coord #[] |>.push (rowC, value))
+  return temp.fold (fun ps k v => ps.push (k, v)) #[]
 
--- todo: remove Nat arg
--- postfix:max "ᵀ" => sparseTranspose
+postfix:max "ᵀ" => sparseTranspose
 
 def printMat (mat : SparseVec Nat (SparseVec Nat Float)) : IO Unit := do
     for (i, row) in mat do
