Tensor/Enumerable.lean
@@ -1,5 +1,7 @@
+-- Kyle Miller
 import Init.Data.Nat.Basic
 import Init.Core
+import Tensor.Has
 
 macro "exfalso" : tactic => `(apply False.elim)
 
@@ -30,7 +32,6 @@ class Enumerable (α : Type u) where
     card : Nat
     enum : α ≃ Fin card
 
-#check Nat.succ_mul
 theorem cartEncodeProp {i j m n : Nat} (hi : i < m) (hj : j < n) : i * n + j < m * n := by
     cases m with
     | zero => exfalso; exact Nat.notLtZero _ hi
@@ -108,3 +109,144 @@ def Enumerable.listOf.aux (α : Type u) [Enumerable α] : Nat -> Nat -> List α
 /-- Create a list of every term in the Enumerable type in order. -/
 def Enumerable.listOf (α : Type u) [Enumerable α] : List α :=
     Enumerable.listOf.aux α 0 (Enumerable.card α)
+
+/-- A function-backed vector -/
+structure Vec (ι : Type u) (α : Type v) where
+    toFun : ι → α
+
+macro "vec" xs:Lean.explicitBinders " => " b:term : term => Lean.expandExplicitBinders `Vec.mk xs b
+
+/-- support `v[i]` notation. -/
+@[inline] def Vec.getOp (self : Vec ι α) (idx : ι) : α := self.toFun idx
+
+/-- A vector as a function mapping indices to values. -/
+class HasVec (β : Type u) (ι : outParam $ Type v) (α : outParam $ Type w) where
+    toVec : β → Vec ι α
+export HasVec (toVec)
+
+instance : HasVec (Vec ι α) ι α := ⟨ id ⟩
+
+instance [Add α] : Add (Vec ι α) where
+    add v w := vec i => v[i] + w[i]
+instance [Sub α] : Sub (Vec ι α) where
+    sub v w := vec i => v[i] - w[i]
+instance [Mul α] : Mul (Vec ι α) where
+    mul v w := vec i => v[i] * w[i]
+instance [Div α] : Div (Vec ι α) where
+    div v w := vec i => v[i] / w[i]
+
+namespace Vec
+
+def push (v : Vec ι (Vec κ α)) : Vec (ι × κ) α := vec p => v[p.1][p.2]
+def pop (v : Vec (ι × κ) α) : Vec ι (Vec κ α) := vec i j => v[(i, j)]
+def reindex (v : Vec ι α) (f : κ → ι) : Vec κ α := vec i => v[f i]
+
+instance [OfNat α n] : OfNat (Vec ι α) n where
+    ofNat := vec i => OfNat.ofNat n
+
+def transpose (v : Vec ι (Vec κ α)) : Vec κ (Vec ι α) := vec j i => v[i][j]
+
+end Vec
+
+def Vec.sum [Enumerable ι] [Add α] [OfNat α Nat.zero] (v : Vec ι α) : α := do
+    let mut s : α := 0
+    for i in Enumerable.listOf ι do
+        s := s + v[i]
+    return s
+
+structure DenseVec (ι : Type u) [Enumerable ι] (α : Type v) where
+    array : Array α
+    hasSize : array.size = Enumerable.card ι
+
+namespace DenseVec
+variable {ι : Type u} [Enumerable ι] {α : Type v}
+
+instance [Repr α] : Repr (DenseVec ι α) where
+    reprPrec d _ := repr d.array
+
+theorem sizeMapEq (a : Array α) (f : α → β) : (a.map f).size = a.size := sorry
+
+instance [HMul α α₁ α₁] : HMul α (DenseVec ι α₁) (DenseVec ι α₁) where
+    hMul r u := ⟨ u.array.map (λ x => r * x) , (sizeMapEq _ _).symm ▸ u.hasSize⟩
+
+def fill (a : α) : DenseVec ι α where
+    array := Array.mkArray (Enumerable.card ι) a
+    hasSize := Array.size_mkArray ..
+
+def empty [Inhabited α] : DenseVec ι α :=
+    fill Inhabited.default
+
+def translateIdx (v : DenseVec ι α) (i : ι) : Fin v.array.size :=
+    let ⟨n, h⟩ := Enumerable.enum i
+    ⟨n, by rw v.hasSize; exact h⟩
+
+/-- Get the value associated to a particular index. -/
+def get (v : DenseVec ι α) (i : ι) : α :=
+    v.array.get (v.translateIdx i)
+
+/-- support `v[i]` notation. -/
+@[inline] def getOp (self : DenseVec ι α) (idx : ι) : α := self.get idx
+
+instance : HasVec (DenseVec ι α) ι α where
+    toVec v := vec i => v[i]
+
+def of [HasVec β ι α] (v : β) : DenseVec ι α where
+    array := do
+        let v' := toVec v
+        let mut a := Array.empty
+        for i in Enumerable.listOf ι do
+            a := a.push $ v'[i]
+        return a
+    hasSize := sorry -- need to define differently to be able to easily prove this
+
+/-- Set the value associated to a particular index. -/
+def set (v : DenseVec ι α) (i : ι) (a : α) : DenseVec ι α where
+    array := v.array.set (v.translateIdx i) a
+    hasSize := by rw [Array.size_set, v.hasSize]
+
+def forIn {α : Type u} {β : Type v} {m : Type v → Type w} [Monad m] (as : DenseVec ι α) (b : β) (f : α → β → m (ForInStep β)) : m β :=
+    as.array.forIn b f
+
+
+instance [HasZero α] [Enumerable ι] : HasZero (DenseVec ι α) where
+    zero := ⟨ Array.mkArray (Enumerable.card ι) HasZero.zero, Array.size_mkArray .. ⟩
+instance [HasZero α] [Enumerable ι] : OfNat (DenseVec ι α) 0 where
+    ofNat := HasZero.zero
+
+def pure (x : α) : DenseVec ι α := fill x
+
+def dot_ (v w : DenseVec ι Float) : Float := do
+    let mut s : Float := 0
+    for i in Enumerable.listOf ι do
+        s := s + v[i] * w[i]
+    return s
+def add_ [Add α] (v w : DenseVec ι α) : DenseVec ι α := do
+    let mut v := v
+    for i in Enumerable.listOf ι do
+        v := v.set i (v.get i + w.get i)
+    return v
+
+-- dsk: alternate add
+def add [Add α] [Inhabited α] ( u v : DenseVec ι α) : DenseVec ι α := do
+    let mut values := u.array
+    for i in [0:values.size] do
+        values := values.set! i (values[i] + v.array[i])
+    return ⟨ values , sorry ⟩
+
+instance [Add α] [Inhabited α]: Add (DenseVec ι α) where
+    add := add
+
+end DenseVec
+
+theorem List.toArraySizeEq (x : List α) : x.toArray.size = x.length := sorry
+
+def List.toDenseVec (x : List α) : DenseVec (Fin x.length) α where
+    array := x.toArray
+    hasSize := List.toArraySizeEq ..
+
+syntax "![" sepBy(term, ", ") "]" : term
+
+macro_rules
+  | `(![ $elems,* ]) => `(List.toDenseVec [ $elems,* ])
+
+example : DenseVec (Fin 3) Nat := ![2,22,222]
